@prefix : <http://purl.org/lis590OD/Fall17/BailOnt#> .
@prefix dc: <http://purl.org/dc/elements/1.1/> .
@prefix tl: <http://purl.org/NET/c4dm/timeline.owl#> .
@prefix dbp: <http://dbpedia.org/resource/> .
@prefix geo: <http://www.w3.org/2003/01/geo/wgs84_pos#> .
@prefix org: <http://www.w3.org/ns/org#> .
@prefix owl: <http://www.w3.org/2002/07/owl#> .
@prefix rdf: <http://www.w3.org/1999/02/22-rdf-syntax-ns#> .
@prefix xml: <http://www.w3.org/XML/1998/namespace> .
@prefix xsd: <http://www.w3.org/2001/XMLSchema#> .
@prefix xsp: <http://www.owl-ontologies.com/2005/08/07/xsp.owl#> .
@prefix foaf: <http://xmlns.com/foaf/0.1/> .
@prefix prov: <http://www.w3.org/ns/prov#> .
@prefix rdfs: <http://www.w3.org/2000/01/rdf-schema#> .
@prefix skos: <http://www.w3.org/2004/02/skos/core#> .
@prefix swrl: <http://www.w3.org/2003/11/swrl#> .
@prefix wped: <http://en.wikipedia.org/wiki/> .
@prefix dolce: <http://ontology.ip.rm.cnr.it/ontologies/DOLCE-Lite#> .
@prefix event: <http://purl.org/NET/c4dm/event.owl#> .
@prefix swrlb: <http://www.w3.org/2003/11/swrlb#> .
@prefix orgrel: <http://purl.org/lis590od/Fall17/OrgRel> .
@prefix dcterms: <http://purl.org/dc/terms/> .
@prefix protege: <http://protege.stanford.edu/plugins/owl/protege#> .
@base <http://purl.org/lis590OD/Fall17/BailOnt> .

<http://purl.org/lis590OD/Fall17/BailOnt> rdf:type owl:Ontology .

#################################################################
#    Object Properties
#################################################################

###  http://purl.org/NET/c4dm/event.owl#agent
event:agent rdf:type owl:ObjectProperty .


###  http://purl.org/NET/c4dm/event.owl#agent_in
event:agent_in rdf:type owl:ObjectProperty ;
               rdfs:domain foaf:Agent ;
               rdfs:range event:Event .


###  http://purl.org/NET/c4dm/event.owl#factor
event:factor rdf:type owl:ObjectProperty .


###  http://purl.org/NET/c4dm/event.owl#factor_of
event:factor_of rdf:type owl:ObjectProperty ;
                rdfs:domain :CaseDefendant ;
                rdfs:range :BailEvent ,
                           :HearingEvent .


###  http://purl.org/lis590OD/Fall17/BailOnt#appearsBefore
:appearsBefore rdf:type owl:ObjectProperty ;
               rdfs:subPropertyOf event:agent ;
               owl:inverseOf :oversees ;
               rdfs:domain :BailEvent ,
                           :HearingEvent ;
               rdfs:range :CourtBranch .


###  http://purl.org/lis590OD/Fall17/BailOnt#attended_by
:attended_by rdf:type owl:ObjectProperty ;
             rdfs:subPropertyOf event:agent ;
             owl:inverseOf :attendee_of ;
             rdfs:domain :BailEvent ,
                         :HearingEvent ;
             rdfs:range :Defendant ,
                        :Judge ;
             rdfs:comment "Inverse property to “attendee_of” object property. This property also relates agent/foaf:person classes to the court events in which they are acting agents. Domain of OrgRel/Court events and range of Person/Judge or Defendant." .


###  http://purl.org/lis590OD/Fall17/BailOnt#attendee_of
:attendee_of rdf:type owl:ObjectProperty ;
             rdfs:subPropertyOf event:agent_in ;
             rdfs:domain foaf:Agent ;
             rdfs:range :HearingEvent ;
             rdfs:comment "The “attendee_of” object property relates agent/foaf:person classes to the court events in which they are acting agents." .


###  http://purl.org/lis590OD/Fall17/BailOnt#bailClearedAt
:bailClearedAt rdf:type owl:ObjectProperty ;
               rdfs:subPropertyOf <http://www.w3.org/2006/time#hasEnd> ;
               rdfs:domain :BailEvent ;
               rdfs:range :BailCleared_Time ;
               rdfs:comment "The “bailClearedTime” object property is the ending time of a BailEvent class instance. The range is a time instance of “BailCleared_Time”." .


###  http://purl.org/lis590OD/Fall17/BailOnt#bailSetAt
:bailSetAt rdf:type owl:ObjectProperty ;
           rdfs:subPropertyOf <http://www.w3.org/2006/time#hasBeginning> ;
           rdfs:domain :BailEvent ;
           rdfs:range :BailSet_Time ;
           rdfs:comment "The “bailSetat” object property relates the BailEvent class to the time instant class BailSet_Time. It is a sub-property of event beginning / beginning times." .


###  http://purl.org/lis590OD/Fall17/BailOnt#defendant_in
:defendant_in rdf:type owl:ObjectProperty ;
              rdfs:subPropertyOf event:agent_in ;
              owl:inverseOf :has_defendent ;
              rdfs:domain :Defendant ;
              rdfs:range :BailEvent ,
                         :HearingEvent ;
              rdfs:comment "The “defendant_in” object property relates the agent/foaf:person of Defendant to the OrgRel events in which they are acting agents." .


###  http://purl.org/lis590OD/Fall17/BailOnt#hasCaseDefendant
:hasCaseDefendant rdf:type owl:ObjectProperty ;
                  rdfs:subPropertyOf event:factor ;
                  owl:inverseOf :isCaseDefendantOf ;
                  rdfs:domain :BailEvent ,
                              :HearingEvent ;
                  rdfs:range :CaseDefendant ;
                  rdfs:comment "Inverse of the “isDefendantOf” object property. The domain of this property is the OrgRel Court events of Bail and Hearing. The range is the CaseDefendant Factor." .


###  http://purl.org/lis590OD/Fall17/BailOnt#has_defendent
:has_defendent rdf:type owl:ObjectProperty ;
               rdfs:subPropertyOf event:agent ;
               rdfs:domain :BailEvent ,
                           :HearingEvent ;
               rdfs:range :Defendant ;
               rdfs:comment "Inverse propery of the “defendant_in” object property. This also relates the agent/foaf:person of Defendant to the OrgRel events in which they are acting agents. Domain is the Event/OrgRel and Range is the Person/Defendant." .


###  http://purl.org/lis590OD/Fall17/BailOnt#hearingBegins
:hearingBegins rdf:type owl:ObjectProperty ;
               rdfs:subPropertyOf <http://www.w3.org/2006/time#hasBeginning> ;
               rdfs:domain :HearingEvent ;
               rdfs:range :Hearing_Time ;
               rdfs:comment "The “hearingBegins” object property relates the HearingEvent class to the time instant class Hearing_Time. It is a sub-property of event beginning / beginning times." .


###  http://purl.org/lis590OD/Fall17/BailOnt#isCaseDefendantOf
:isCaseDefendantOf rdf:type owl:ObjectProperty ;
                   rdfs:subPropertyOf event:factor_of ;
                   rdfs:domain :CaseDefendant ;
                   rdfs:range :BailEvent ,
                              :HearingEvent ;
                   rdfs:comment "The “isDefendantOf” object property relates the factor class of CaseDefandant to the OrgRel Events in which they are a factor. Ex. the person “Jim” as the defendant factor/topic of a BailEvent." .


###  http://purl.org/lis590OD/Fall17/BailOnt#isPresided_by
:isPresided_by rdf:type owl:ObjectProperty ;
               rdfs:subPropertyOf event:agent_in ;
               owl:inverseOf :presides_over ;
               rdfs:domain :HearingEvent ;
               rdfs:range :Judge ;
               rdfs:comment "The “ispresides_by” object property relates Domain of OrgRel event, to the Judge that is the agent_in that event." .


###  http://purl.org/lis590OD/Fall17/BailOnt#oversees
:oversees rdf:type owl:ObjectProperty ;
          rdfs:subPropertyOf event:agent_in ;
          rdfs:domain :CourtBranch ;
          rdfs:range :BailEvent ,
                     :HearingEvent .


###  http://purl.org/lis590OD/Fall17/BailOnt#presides_over
:presides_over rdf:type owl:ObjectProperty ;
               rdfs:subPropertyOf event:agent ;
               rdfs:domain :Judge ;
               rdfs:range :HearingEvent ;
               rdfs:comment "The “presides_over” object property relates the Judge to the OrgRel event in which they are an agent." .


###  http://www.w3.org/2006/time#hasBeginning
<http://www.w3.org/2006/time#hasBeginning> rdf:type owl:ObjectProperty ;
                                           rdfs:domain :HearingEvent .


###  http://www.w3.org/2006/time#hasEnd
<http://www.w3.org/2006/time#hasEnd> rdf:type owl:ObjectProperty .


#################################################################
#    Classes
#################################################################

###  http://purl.org/NET/c4dm/event.owl#Event
event:Event rdf:type owl:Class .


###  http://purl.org/NET/c4dm/event.owl#Factor
event:Factor rdf:type owl:Class .


###  http://purl.org/lis590OD/Fall17/BailOnt#BailCleared_Time
:BailCleared_Time rdf:type owl:Class ;
                  rdfs:subClassOf <http://www.w3.org/2006/time#Instant> ;
                  rdfs:comment "The “BailCleared_Time” is a subclass of time instances. If this time exists it can be inferred that a hearing was attended and a BailEvent is over." .


###  http://purl.org/lis590OD/Fall17/BailOnt#BailEvent
:BailEvent rdf:type owl:Class ;
           rdfs:subClassOf <http://purl.org/lis590od/Fall17/OrgRel#OrganizationRelationship> ,
                           [ rdf:type owl:Restriction ;
                             owl:onProperty :bailSetAt ;
                             owl:someValuesFrom :BailSet_Time
                           ] ,
                           [ rdf:type owl:Restriction ;
                             owl:onProperty :hasCaseDefendant ;
                             owl:someValuesFrom :CaseDefendant
                           ] ;
           rdfs:comment "The \"BailEvent\" is the main bail construction. It starts when the bail is set and ends when the bail is cleared (upon hearing attendance) or forfeit (upon hearing non-attendance)" .


###  http://purl.org/lis590OD/Fall17/BailOnt#BailSet_Time
:BailSet_Time rdf:type owl:Class ;
              rdfs:subClassOf <http://www.w3.org/2006/time#Instant> ;
              rdfs:comment "The “BailSet_Time” is a subclass of time instances. If this time exists it starts a BailEvent." .


###  http://purl.org/lis590OD/Fall17/BailOnt#CaseDefendant
:CaseDefendant rdf:type owl:Class ;
               rdfs:subClassOf event:Factor ;
               rdfs:comment "The “CaseDefendant” is the topic or factor of a hearing or bail event. This is not a subclass of person." .


###  http://purl.org/lis590OD/Fall17/BailOnt#CourtAppearence_Time
:CourtAppearence_Time rdf:type owl:Class ;
                      rdfs:subClassOf <http://www.w3.org/2006/time#Instant> ;
                      rdfs:comment "The “CourtApperance_Time” is a subclass of time instances and a superclass to Hearing_Time and possibly an Arraignment time could be integrated at this level." .


###  http://purl.org/lis590OD/Fall17/BailOnt#CourtBranch
:CourtBranch rdf:type owl:Class ;
             rdfs:subClassOf foaf:Organization ;
             rdfs:comment "The “CourtBranch” class is a subclass of organization and refers to the kind of court in which the hearing will be seen. Traffic court, etc." .


###  http://purl.org/lis590OD/Fall17/BailOnt#Defendant
:Defendant rdf:type owl:Class ;
           rdfs:subClassOf foaf:Person ;
           rdfs:comment "The “Defendant” is the agent which can take actions in the OrgRel events. BailEvent and HearingEvent." .


###  http://purl.org/lis590OD/Fall17/BailOnt#HearingEvent
:HearingEvent rdf:type owl:Class ;
              rdfs:subClassOf <http://purl.org/lis590od/Fall17/OrgRel#OrganizationRelationship> ,
                              [ rdf:type owl:Restriction ;
                                owl:onProperty :hasCaseDefendant ;
                                owl:someValuesFrom :CaseDefendant
                              ] ,
                              [ rdf:type owl:Restriction ;
                                owl:onProperty :hearingBegins ;
                                owl:someValuesFrom :Hearing_Time
                              ] ;
              rdfs:comment "The “HearingEvent” is the court event at which the defendant is an agent and over which the judge presides. It is a organization relationship between the court system, the defendant, and other active agents." .


###  http://purl.org/lis590OD/Fall17/BailOnt#Hearing_Time
:Hearing_Time rdf:type owl:Class ;
              rdfs:subClassOf :CourtAppearence_Time ;
              rdfs:comment "The “Hearing_Time” is a subclass of CourtApperance_Time. It is the scheduled time of the HearingEvent." .


###  http://purl.org/lis590OD/Fall17/BailOnt#Judge
:Judge rdf:type owl:Class ;
       rdfs:subClassOf foaf:Person ;
       rdfs:comment "The “Judge” is a class of persons that set bails and preside over hearings." .


###  http://purl.org/lis590od/Fall17/OrgRel#OrganizationRelationship
<http://purl.org/lis590od/Fall17/OrgRel#OrganizationRelationship> rdf:type owl:Class ;
                                                                  rdfs:subClassOf event:Event .


###  http://www.w3.org/2006/time#Instant
<http://www.w3.org/2006/time#Instant> rdf:type owl:Class .


###  http://xmlns.com/foaf/0.1/Agent
foaf:Agent rdf:type owl:Class .


###  http://xmlns.com/foaf/0.1/Organization
foaf:Organization rdf:type owl:Class ;
                  rdfs:subClassOf foaf:Agent .


###  http://xmlns.com/foaf/0.1/Person
foaf:Person rdf:type owl:Class .


###  Generated by the OWL API (version 4.2.8.20170104-2310) https://github.com/owlcs/owlapi
